Iteration on the microstep semantics.

Language.v
@@ -1,172 +1,315 @@
-Require Import Coq.Logic.Classical.
-Require Import Coq.Logic.FunctionalExtensionality.
-Require Import Coq.Logic.PropExtensionality.
+ Require Import Coq.Logic.Classical.
+ Require Import Coq.Logic.FunctionalExtensionality.
+ Require Import Coq.Logic.PropExtensionality.
+ 
+ Require Import Coq.Arith.PeanoNat.
+ Require Import Coq.Lists.List.
+ 
+ Import ListNotations.
+ 
+ Section Syntax.
+ 
+ (* Variables *)
+ Definition var := nat.
+ Definition var_dec (x y: var): {x = y} + {x <> y} := Nat.eq_dec x y.
+ 
+ (* Program signature *)
+ Class Signature :=
+ { Prim: Set
+ ; Test: Set
+ ; Paccess: Prim -> list var
+ ; Pchange: Prim -> list var
+ ; Taccess: Test -> list var
+ }.
+ 
+ Context {Sigma: Signature}.
+ 
+ (* Programs *)
+ Inductive program :=
+ | prim: Prim -> program
+ | skip: program
+ | halt: program
+ | local: var -> program -> program
+ | comp: program -> program -> program
+ | ite: Test -> program -> program -> program
+ | while: Test -> program -> program.
+ 
+ Fixpoint access (S: program): list var :=
+   match S with
+   | prim O1 => Paccess O1
+   | skip => []
+   | halt => []
+   | local x S1 => remove var_dec x (access S1)
+   | comp S1 S2 => access S1 ++ access S2
+   | ite T S1 S2 => Taccess T ++ access S1 ++ access S2
+   | while T S1 => Taccess T ++ access S1
+   end.
+ 
+ Fixpoint change (S: program): list var :=
+   match S with
+   | prim O1 => Pchange O1
+   | skip => []
+   | halt => []
+   | local x S1 => remove var_dec x (change S1)
+   | comp S1 S2 => change S1 ++ change S2
+   | ite T S1 S2 => change S1 ++ change S2
+   | while T S1 => change S1
+   end.
+ 
+ End Syntax.
+ 
+ Print program.
+ 
+ Section SemanticBasis.
+ 
+ Class Domain := { A: Set }.
+ 
+ Context {D: Domain}.
+ 
+ (* Semantic domain: relations on state *)
+ Definition state := var -> A.
+ Definition state_eq (f g: state) := functional_extensionality f g.
+ (* state update *)
+ Definition update (f: state) (x: var) (a: A): state :=
+   fun y => if var_dec x y then a else f y.
+ (* f and g differ in the variables xs *)
+ Definition diff (f g: state) (xs: list var): Prop :=
+   forall x, ~In x xs -> f x = g x.
+ (* f and g are the same in the variables xs *)
+ Definition same (f g: state) (xs : list var): Prop :=
+   forall x, In x xs -> f x = g x.
+ Proposition same_refl f xs: same f f xs.
+ unfold same; auto.
+ Qed.
+ 
+ Context {Sigma: Signature}.
+ 
+ Class Interp :=
+ { Prel (O: Prim): state -> state -> Prop
+ ; Prel_change O s t: Prel O s t -> diff s t (Pchange O)
+ ; Prel_access O s t s': Prel O s t -> same s s' (Paccess O) -> exists t', Prel O s' t'
+ ; Prel_det O s t s' t': Prel O s t -> Prel O s' t' -> same s s' (Paccess O) -> same t t' (Pchange O)
+ ; Tset (T: Test): state -> Prop
+ ; Tset_access T s s': same s s' (Taccess T) -> Tset T s -> Tset T s'
+ ; Tset_dec T s: {Tset T s} + {~Tset T s}
+ }.
+ 
+ Context {I: Interp}.
+ 
+ Proposition Prel_access' O s t s':
+   Prel O s t -> same s s' (Paccess O) -> exists t', Prel O s' t' /\ same t t' (Pchange O).
+ intros.
+ pose proof (Prel_access O s t s' H H0).
+ destruct H1 as (t' & H1).
+ exists t'. split; auto.
+ eapply Prel_det. apply H. apply H1. auto.
+ Qed.
+ 
+ Lemma Interp_determinism O s t t':
+   Prel O s t -> Prel O s t' -> t = t'.
+ intros; apply state_eq; intros.
+ (* either x is in change or not *)
+ destruct (In_dec var_dec x (Pchange O)).
+ - pose proof (Prel_det _ _ _ _ _ H H0 (same_refl _ _)).
+   apply H1; auto.
+ - pose proof (Prel_change _ _ _ H).
+   pose proof (Prel_change _ _ _ H0).
+   unfold diff in H1, H2.
+   rewrite <- H1; auto.
+ Qed.
+ 
+ End SemanticBasis.
+ 
+ Section SmallStepSemantics.
+ 
+ Context {Sigma: Signature}.
+ Context {D: Domain}.
+ 
+ (* We need an interpretation in which there are `restore' operations. *)
+ 
+ Class InterpRestore (I: Interp) :=
+ { Prim_restore (x: var) (a: A): Prim
+ ; Prim_restore_spec a x s: Prel (Prim_restore x a) s (update s x a) }.
+ 
+ Context {I: Interp}.
+ Context {I1: InterpRestore I}.
+ 
+ Definition config := (program * state)%type.
+ 
+ Inductive smallstep: config -> config -> Prop :=
+ | SSprim O s t: Prel O s t -> smallstep (prim O, s) (skip, t)
+ | SSskip s: smallstep (skip, s) (skip, s)
+ | SShalt s: smallstep (halt, s) (halt, s)
+ | SSlocal x S1 s: smallstep (local x S1, s) (comp S1 (prim (Prim_restore x (s x))), s)
+ | SScomp S1 S2 s t: smallstep (S1, s) (skip, t) -> smallstep (comp S1 S2, s) (S2, t)
+ | SScomp' S1 S1' S2 s t: S1' <> skip -> smallstep (S1, s) (S1', t) -> smallstep (comp S1 S2, s) (comp S1' S2, t)
+ | SSite1 T S1 S2 s: Tset T s -> smallstep (ite T S1 S2, s) (S1, s)
+ | SSite2 T S1 S2 s: ~Tset T s -> smallstep (ite T S1 S2, s) (S2, s)
+ | SSwhile T S1 s: Tset T s -> smallstep (while T S1, s) (comp S1 (while T S1), s)
+ | SSwhile' T S1 s: ~Tset T s -> smallstep (while T S1, s) (skip, s).
+ 
+ Lemma determinism: forall c c' c'', smallstep c c' /\ smallstep c c'' -> c' = c''.
+ intros.
+ destruct H.
+ destruct c.
+ generalize dependent c'';
+ generalize dependent c';
+ generalize dependent s.
+ induction p; intros;
+ try (inversion H; inversion H0; try contradiction; reflexivity).
+ (* base case *)
+ + inversion H; inversion H0; f_equal.
+   apply (Interp_determinism p s t t0); auto.
+ (* sequential composition *)
+ + inversion H; inversion H0.
+   - pose proof (IHp1 _ _ H5 _ H10).
+     inversion H11; auto.
+   - pose proof (IHp1 _ _ H5 _ H11).
+     inversion H12. exfalso. firstorder.
+   - pose proof (IHp1 _ _ H6 _ H11).
+     inversion H12. exfalso. firstorder.
+   - pose proof (IHp1 _ _ H6 _ H12).
+     inversion H13; auto.
+ Qed.
+ 
+ Inductive bigstep : program -> state -> state -> Prop := 
+   | BSprim O s t: Prel O s t -> bigstep (prim O) s t 
+   | BScomp S1 S2 s t s': bigstep S1 s s' -> bigstep S2 s' t -> bigstep (comp S1 S2) s t.
 
-Require Import Coq.Arith.PeanoNat.
-Require Import Coq.Lists.List.
 
-Import ListNotations.
+ Section Micro.
 
-Section Syntax.
 
-(* Variables *)
-Definition var := nat.
-Definition var_dec (x y: var): {x = y} + {x <> y} := Nat.eq_dec x y.
+ Inductive microprogram : Set :=
+   | mprog : program -> microprogram
+   | mpar : microprogram -> microprogram -> microprogram
+   | mchoice : microprogram -> microprogram -> microprogram
+   | massert : Test -> microprogram.
 
-(* Program signature *)
-Class Signature :=
-{ Prim: Set
-; Test: Set
-; Paccess: Prim -> list var
-; Pchange: Prim -> list var
-; Taccess: Test -> list var
-}.
+   Coercion mprog : program >-> microprogram.
 
-Context {Sigma: Signature}.
+ Definition microconfig : Set := (microprogram*state)%type.
+ 
+ (*
+    (A1;A2) + B  --> A1; (A2 + (A1^-1);B)
+    I(A1;A1^-1;B) = I(B)
+    (A1;A1^-1, s) ->* (A1^-1, t) ->* (skip, s)
+  *)
+ Class InterpReverse `(I: InterpRestore) :=
+ { 
+   Prim_reverse (p : Prim) (s : state): Prim
+   ; Prim_reverse_spec p s t: Prel p s t  -> Prel (Prim_reverse p s) t s }.
 
-(* Programs *)
-Inductive program :=
-| prim: Prim -> program
-| skip: program
-| halt: program
-| local: var -> program -> program
-| comp: program -> program -> program
-| ite: Test -> program -> program -> program
-| while: Test -> program -> program.
+ Context {I2: InterpReverse I1}.
+ (*
+  Properties:
+    identities of reverse composition
+    sequential reverse
+    branch and reverse
+    ite b S1 S2 -> if b then (S1; S2) else S3 -(b true)-> S1; S2 -(in s)-> (S2, s') -(b false)-> S1^-1; S3 
+      (S1, s) -> (skip, s')
+    reverse o reverse = id ?
 
-Fixpoint access (S: program): list var :=
-  match S with
-  | prim O1 => Paccess O1
-  | skip => []
-  | halt => []
-  | local x S1 => remove var_dec x (access S1)
-  | comp S1 S2 => access S1 ++ access S2
-  | ite T S1 S2 => Taccess T ++ access S1 ++ access S2
-  | while T S1 => Taccess T ++ access S1
-  end.
+ *)
 
-Fixpoint change (S: program): list var :=
-  match S with
-  | prim O1 => Pchange O1
-  | skip => []
-  | halt => []
-  | local x S1 => remove var_dec x (change S1)
-  | comp S1 S2 => change S1 ++ change S2
-  | ite T S1 S2 => change S1 ++ change S2
-  | while T S1 => change S1
-  end.
+ Inductive branchfree_program : Set :=
+  | bfprim : Prim -> branchfree_program
+  | bfskip : branchfree_program
+  | bfhalt : branchfree_program
+  | bflocal : var -> branchfree_program -> branchfree_program
+  | bfcomp : branchfree_program -> branchfree_program -> branchfree_program.
 
-End Syntax.
+ Fixpoint prog (bf : branchfree_program) : program :=
+   match bf with
+   | bfprim S1 => prim S1 
+   | bfskip => skip
+   | bfhalt => halt
+   | bflocal n S1 => local n (prog S1)
+   | bfcomp S1 S2 => comp (prog S1) (prog S2)
+   end.
 
-Print program.
+ Coercion prog : branchfree_program >-> program.
 
-Section SemanticBasis.
+ Definition isInvertible (p : program) : Prop :=
+  exists p',  forall s t, bigstep p s t  -> bigstep p' t s.
 
-Class Domain := { A: Set }.
+ Definition isReversible (p : program) (s : state) (rev_p : program) : Prop :=
+  forall t, bigstep p s t  -> bigstep rev_p t s.
 
-Context {D: Domain}.
+ (*
+ Inductive reverse (p : branchfree_program) (s : state) : branchfree_program :=
+   match p with
+   | bfprim S1 => bfprim (Prim_reverse S1 s)
+   | bfskip => bfskip
+   | bfhalt => bfhalt
+   | bflocal n S1 => bflocal n (reverse S1 s) 
+   | bfcomp S1 S2 => bfcomp (reverse S2 s) (reverse S1 s)
+   end.
+  *)
 
-(* Semantic domain: relations on state *)
-Definition state := var -> A.
-Definition state_eq (f g: state) := functional_extensionality f g.
-(* state update *)
-Definition update (f: state) (x: var) (a: A): state :=
-  fun y => if var_dec x y then a else f y.
-(* f and g differ in the variables xs *)
-Definition diff (f g: state) (xs: list var): Prop :=
-  forall x, ~In x xs -> f x = g x.
-(* f and g are the same in the variables xs *)
-Definition same (f g: state) (xs : list var): Prop :=
-  forall x, In x xs -> f x = g x.
-Proposition same_refl f xs: same f f xs.
-unfold same; auto.
-Qed.
 
-Context {Sigma: Signature}.
+ Lemma bf_reversibility : forall p s, exists rev_p, isReversible p s rev_p. 
+ (*
+    reverse (ite b S1 S2) = if (exists b') then (reverse S1) else (reverse S2) where b' is true in final state if b was true in initial state.
+  *)
+ Admitted.
 
-Class Interp :=
-{ Prel (O: Prim): state -> state -> Prop
-; Prel_change O s t: Prel O s t -> diff s t (Pchange O)
-; Prel_access O s t s': Prel O s t -> same s s' (Paccess O) -> exists t', Prel O s' t'
-; Prel_det O s t s' t': Prel O s t -> Prel O s' t' -> same s s' (Paccess O) -> same t t' (Pchange O)
-; Tset (T: Test): state -> Prop
-; Tset_access T s s': same s s' (Taccess T) -> Tset T s -> Tset T s'
-; Tset_dec T s: {Tset T s} + {~Tset T s}
-}.
+ (*
+ ...
 
-Context {I: Interp}.
+    reverse (x:=-1; x^2) (x -> 10) =
+    reverse x^2 (x -> -1); (reverse x:=-1 (x->10))
 
-Proposition Prel_access' O s t s':
-  Prel O s t -> same s s' (Paccess O) -> exists t', Prel O s' t' /\ same t t' (Pchange O).
-intros.
-pose proof (Prel_access O s t s' H H0).
-destruct H1 as (t' & H1).
-exists t'. split; auto.
-eapply Prel_det. apply H. apply H1. auto.
-Qed.
 
-Lemma Interp_determinism O s t t':
-  Prel O s t -> Prel O s t' -> t = t'.
-intros; apply state_eq; intros.
-(* either x is in change or not *)
-destruct (In_dec var_dec x (Pchange O)).
-- pose proof (Prel_det _ _ _ _ _ H H0 (same_refl _ _)).
-  apply H1; auto.
-- pose proof (Prel_change _ _ _ H).
-  pose proof (Prel_change _ _ _ H0).
-  unfold diff in H1, H2.
-  rewrite <- H1; auto.
-Qed.
+          (x -> 10) s [p]
+          x:=-1;
+          ||  /\?
+          \/  || 
+          x:=x^2;   
+          (x -> 1, p') t [p']
+          x:=10;
+          (x -> 10) s
 
-End SemanticBasis.
+  Cost of speculation: cheapest program to revert (time/space).
+  *)
 
-Section SmallStepSemantics.
 
-Context {Sigma: Signature}.
-Context {D: Domain}.
 
-(* We need an interpretation in which there are `restore' operations. *)
+ Inductive microstep: microconfig -> microconfig -> Prop :=
+ | MSmprog S S' s t: smallstep (S, s) (S', t) -> microstep (mprog S, s) (mprog S', t)
+ | MSmparl S1 S2 S1' s t: microstep (S1, s) (S1', t) -> microstep (mpar S1 S2, s) (mpar S1' S2, t) 
+ | MSmparr S1 S2 S2' s t: microstep (S2, s) (S2', t) -> microstep (mpar S1 S2, s) (mpar S1  S2', t) 
+     (* | MSmchoice S1 S1' S2 RevS s s' t: isReversible S1 s RevS -> microstep (mprog S1, s) (S1', s') -> 
+                                               microstep (mchoice S1 S2, s) 
+        (mchoice S1' (comp RevS S2), t) *).
+     
 
-Class InterpRestore (I: Interp) :=
-{ Prim_restore (x: var) (a: A): Prim
-; Prim_restore_spec a x s: Prel (Prim_restore x a) s (update s x a) }.
+ Record measures {A : Type} : Type := 
+   {
+   resource: list (A -> nat) (* list of operations *) 
+   }.
 
-Context `{I: InterpRestore}.
 
-Definition config := (program * state)%type.
+ (*
+   
+  *)
 
-Inductive smallstep: config -> config -> Prop :=
-| SSprim O s t: Prel O s t -> smallstep (prim O, s) (skip, t)
-| SSskip s: smallstep (skip, s) (skip, s)
-| SShalt s: smallstep (halt, s) (halt, s)
-| SSlocal x S1 s: smallstep (local x S1, s) (comp S1 (prim (Prim_restore x (s x))), s)
-| SScomp S1 S2 s t: smallstep (S1, s) (skip, t) -> smallstep (comp S1 S2, s) (S2, t)
-| SScomp' S1 S1' S2 s t: S1' <> skip -> smallstep (S1, s) (S1', t) -> smallstep (comp S1 S2, s) (comp S1' S2, t)
-| SSite1 T S1 S2 s: Tset T s -> smallstep (ite T S1 S2, s) (S1, s)
-| SSite2 T S1 S2 s: ~Tset T s -> smallstep (ite T S1 S2, s) (S2, s)
-| SSwhile T S1 s: Tset T s -> smallstep (while T S1, s) (comp S1 (while T S1), s)
-| SSwhile' T S1 s: ~Tset T s -> smallstep (while T S1, s) (skip, s).
+ Definition measure : microprogram -> nat -> measure 
 
-Lemma determinism: forall c c' c'', smallstep c c' /\ smallstep c c'' -> c' = c''.
-intros.
-destruct H.
-destruct c.
-generalize dependent c'';
-generalize dependent c';
-generalize dependent s.
-induction p; intros;
-try (inversion H; inversion H0; try contradiction; reflexivity).
-(* base case *)
-+ inversion H; inversion H0; f_equal.
-  apply (Interp_determinism p s t t0); auto.
-(* sequential composition *)
-+ inversion H; inversion H0.
-  - pose proof (IHp1 _ _ H5 _ H10).
-    inversion H11; auto.
-  - pose proof (IHp1 _ _ H5 _ H11).
-    inversion H12. exfalso. firstorder.
-  - pose proof (IHp1 _ _ H6 _ H11).
-    inversion H12. exfalso. firstorder.
-  - pose proof (IHp1 _ _ H6 _ H12).
-    inversion H13; auto.
-Qed.
+ Record wf_microprogram : Set :=
+   {|
+      mp : microprogram;
+      wf_par : 
+   |}
+
+ Inductive microstep : program -> 
+
+
+       
+
+
+
+
+
+
+
